ArkLib/OracleReduction/Composition/Sequential/ProtocolSpec.lean
@@ -7,6 +7,7 @@ Authors: Quang Dao
 import ArkLib.ToMathlib.BigOperators.Fin
 import ArkLib.OracleReduction.ProtocolSpec
 import ArkLib.OracleReduction.Cast
+import ArkLib.Data.Fin.Tuple.Lemmas
 
 /-! # Sequential Composition of Protocol Specifications
 
@@ -21,18 +22,17 @@ variable {m n : ℕ}
 
 /-- Adding a round with direction `dir` and type `Message` to the beginning of a `ProtocolSpec` -/
 abbrev cons (pSpec : ProtocolSpec n) (dir : Direction) (Message : Type) :
-    ProtocolSpec (n + 1) := Fin.cons ⟨dir, Message⟩ pSpec
+    ProtocolSpec (n + 1) :=
+  ⟨FinVec.cons dir pSpec.dir, FinVec.cons Message pSpec.Type⟩
 
-/-- Adding a round with direction `dir` and type `Message` to the end of a `ProtocolSpec` -/
-abbrev snoc (pSpec : ProtocolSpec n) (dir : Direction) (Message : Type) :
-    ProtocolSpec (n + 1) := Fin.snoc pSpec ⟨dir, Message⟩
+/-- Concatenate a round with direction `dir` and type `Message` to the end of a `ProtocolSpec` -/
+abbrev concat (pSpec : ProtocolSpec n) (dir : Direction) (Message : Type) :
+    ProtocolSpec (n + 1) :=
+  ⟨FinVec.concat pSpec.dir dir, FinVec.concat pSpec.Type Message⟩
 
 /-- Appending two `ProtocolSpec`s -/
 abbrev append (pSpec : ProtocolSpec m) (pSpec' : ProtocolSpec n) : ProtocolSpec (m + n) :=
-  Fin.append pSpec pSpec'
-
-@[inline, reducible]
-def mkSingle (dir : Direction) (Message : Type) : ProtocolSpec 1 := fun _ => ⟨dir, Message⟩
+  ⟨FinVec.append pSpec.dir pSpec'.dir, FinVec.append pSpec.Type pSpec'.Type⟩
 
 @[inherit_doc]
 infixl : 65 " ++ₚ " => ProtocolSpec.append
@@ -41,21 +41,35 @@ infixl : 65 " ++ₚ " => ProtocolSpec.append
 theorem append_cast_left {n m : ℕ} {pSpec : ProtocolSpec n} {pSpec' : ProtocolSpec m} (n' : ℕ)
     (h : n + m = n' + m) :
       dcast h (pSpec ++ₚ pSpec') = (dcast (Nat.add_right_cancel h) pSpec) ++ₚ pSpec' := by
-  simp [append, dcast, ProtocolSpec.cast, Fin.append_cast_left]
+  simp only [append, dcast, ProtocolSpec.cast, FinVec.append_eq_fin_append]
+  simp
 
 @[simp]
 theorem append_cast_right {n m : ℕ} (pSpec : ProtocolSpec n) (pSpec' : ProtocolSpec m) (m' : ℕ)
     (h : n + m = n + m') :
       dcast h (pSpec ++ₚ pSpec') = pSpec ++ₚ (dcast (Nat.add_left_cancel h) pSpec') := by
-  simp [append, dcast, ProtocolSpec.cast, Fin.append_cast_right]
+  simp only [append, dcast, ProtocolSpec.cast, FinVec.append_eq_fin_append, Fin.append_cast_right]
 
 theorem append_left_injective {pSpec : ProtocolSpec n} :
-    Function.Injective (@ProtocolSpec.append m n · pSpec) :=
-  Fin.append_left_injective pSpec
+    Function.Injective (@ProtocolSpec.append m n · pSpec) := by
+  simp only [append, FinVec.append_eq_fin_append]
+  intro x y h
+  simp at h
+  obtain ⟨hDir, hType⟩ := h
+  ext i
+  · simp [Fin.append_left_injective pSpec.dir hDir]
+  · simp [Fin.append_left_injective pSpec.Type hType]
 
 theorem append_right_injective {pSpec : ProtocolSpec m} :
-    Function.Injective (@ProtocolSpec.append m n pSpec) :=
-  Fin.append_right_injective pSpec
+    Function.Injective (@ProtocolSpec.append m n pSpec) := by
+  unfold ProtocolSpec.append
+  simp only [FinVec.append_eq_fin_append]
+  intro x y h
+  simp at h
+  obtain ⟨hDir, hType⟩ := h
+  ext i
+  · simp [Fin.append_right_injective pSpec.dir hDir]
+  · simp [Fin.append_right_injective pSpec.Type hType]
 
 @[simp]
 theorem append_left_cancel_iff {pSpec : ProtocolSpec n} {p1 p2 : ProtocolSpec m} :
@@ -69,40 +83,49 @@ theorem append_right_cancel_iff {pSpec : ProtocolSpec m} {p1 p2 : ProtocolSpec n
 
 @[simp]
 theorem snoc_take {pSpec : ProtocolSpec n} (k : ℕ) (h : k < n) :
-    (pSpec.take k (Nat.le_of_succ_le h) ++ₚ (fun (_ : Fin 1) => pSpec ⟨k, h⟩))
+    (pSpec.take k (Nat.le_of_succ_le h) ++ₚ ⟨![pSpec.dir ⟨k, h⟩], ![pSpec.Type ⟨k, h⟩]⟩)
       = pSpec.take (k + 1) h := by
-  simp only [append, take, Fin.append_right_eq_snoc, Fin.take_succ_eq_snoc]
+  simp only [append, take, FinVec.append_eq_fin_append, Fin.append_right_eq_snoc,
+    Fin.take_succ_eq_snoc]
+  ext : 1 <;> simp
 
 variable {pSpec₁ : ProtocolSpec m} {pSpec₂ : ProtocolSpec n}
 
 @[simp]
 theorem take_append_left :
     (pSpec₁ ++ₚ pSpec₂).take m (Nat.le_add_right m n) = pSpec₁ := by
-  simp only [take, append]
-  ext i : 1
-  have : Fin.castLE (by omega) i = Fin.castAdd n i := rfl
-  simp [Fin.take_apply, Fin.append_left, this]
+  simp only [take, FinVec.append_eq_fin_append]
+  ext <;> simp [Fin.take_apply]
 
 @[simp]
 theorem rtake_append_right :
     (pSpec₁ ++ₚ pSpec₂).rtake n (Nat.le_add_left n m) = pSpec₂ := by
-  simp only [rtake, append]
-  ext i : 1
-  simp [Fin.rtake_apply, Fin.append_right]
+  simp only [rtake, FinVec.append_eq_fin_append]
+  ext i : 2 <;> simp [Fin.rtake, Fin.append_right]
 
 namespace Transcript
 
 variable {k : Fin (m + n + 1)}
 
-/-- The first half of a partial transcript for a concatenated protocol. -/
+/-- The first half of a partial transcript for a concatenated protocol, up to round `k < m + n + 1`.
+
+This is defined to be the full transcript for the first half if `k ≥ m`. -/
 def fst (T : (pSpec₁ ++ₚ pSpec₂).Transcript k) : pSpec₁.Transcript ⟨min k m, by omega⟩ :=
-  fun i => sorry
-  -- cast T i
+  if hk : k ≤ m then
+    fun i => by
+    dsimp [take]; have := T ⟨i, lt_of_lt_of_le i.isLt (inf_le_left)⟩; simp at this; sorry
+    -- dcast (by sorry) (T ⟨i, lt_of_lt_of_le i.isLt (inf_le_left)⟩)
+  else
+    fun i => sorry
+    -- dcast (by sorry) (T ⟨i, by omega⟩)
 
 /-- The second half of a partial transcript for a concatenated protocol. -/
 def snd (T : (pSpec₁ ++ₚ pSpec₂).Transcript k) : pSpec₂.Transcript ⟨k - m, by omega⟩ :=
-  fun i => sorry
-  -- cast T i
+  if hk : k ≤ m then
+    fun i => Fin.elim0 (by simpa [hk] using i)
+  else
+    fun i => sorry
+    -- dcast (by sorry) (T ⟨m + i, by simp_all; dsimp at i; have := i.isLt; omega⟩)
 
 end Transcript
 
@@ -110,17 +133,19 @@ namespace FullTranscript
 
 /-- Appending two transcripts for two `ProtocolSpec`s -/
 def append (T₁ : FullTranscript pSpec₁) (T₂ : FullTranscript pSpec₂) :
-    FullTranscript (pSpec₁ ++ₚ pSpec₂) :=
-  fun i => (Fin.append_comp' Prod.snd i).mp (Fin.addCases' T₁ T₂ i)
+    FullTranscript (pSpec₁ ++ₚ pSpec₂) := by
+  dsimp [FullTranscript]
+  convert FinTuple.append T₁ T₂
+  -- fun i => (FinVec.append Prod.snd i).mp (Fin.addCases' T₁ T₂ i)
 
 @[inherit_doc]
 infixl : 65 " ++ₜ " => append
 
 /-- Adding a message with a given direction and type to the end of a `Transcript` -/
-def snoc {pSpec : ProtocolSpec n} {NextMessage : Type}
+def concat {pSpec : ProtocolSpec n} {NextMessage : Type}
     (T : FullTranscript pSpec) (dir : Direction) (msg : NextMessage) :
-        FullTranscript (pSpec ++ₚ .mkSingle dir NextMessage) :=
-  append T fun _ => msg
+        FullTranscript (pSpec ++ₚ ⟨!v[dir], !v[NextMessage]⟩) :=
+  append T (fun _ => msg)
 
 -- TODO: fill
 
@@ -143,51 +168,51 @@ theorem take_append_left (T : FullTranscript pSpec₁) (T' : FullTranscript pSpe
     (T ++ₜ T').take m (Nat.le_add_right m n) =
       T.cast rfl (by simp [ProtocolSpec.append]) := by
   ext i
-  simp [take, append, ProtocolSpec.append, Fin.castLE, Fin.addCases', Fin.addCases,
-    FullTranscript.cast, Transcript.cast]
+  simp [take, append, ProtocolSpec.append, Fin.castLE,
+    FullTranscript.cast, Transcript.cast]; sorry
 
 @[simp]
 theorem rtake_append_right (T : FullTranscript pSpec₁) (T' : FullTranscript pSpec₂) :
     (T ++ₜ T').rtake n (Nat.le_add_left n m) =
       T'.cast rfl (by simp [ProtocolSpec.append]) := by
   ext i
-  simp only [ProtocolSpec.append, getType, Fin.rtake_apply, Fin.natAdd, Fin.cast_mk, rtake, append,
-    Fin.addCases', Fin.addCases, add_tsub_cancel_right, add_lt_iff_neg_left, not_lt_zero',
-    ↓reduceDIte, Fin.subNat_mk, Fin.natAdd_mk, eq_mpr_eq_cast, eq_mp_eq_cast, FullTranscript.cast,
-    Transcript.cast, Fin.val_last, Fin.cast_eq_self, Fin.castLE_refl]
-  have : m + n - n + i.val - m = i.val := by omega
-  rw! (castMode := .all) [this]
-  simp [eqRec_eq_cast]
+  simp [rtake, Fin.rtake, append, Fin.cast, FullTranscript.cast, Transcript.cast]
+  sorry
+  -- have : m + n - n + i.val - m = i.val := by omega
+  -- rw! (castMode := .all) [this]
+  -- simp [eqRec_eq_cast]
 
 /-- The first half of a transcript for a concatenated protocol -/
 def fst (T : FullTranscript (pSpec₁ ++ₚ pSpec₂)) : FullTranscript pSpec₁ :=
   fun i => by
-    simpa [ProtocolSpec.append, Fin.append_left] using T (Fin.castAdd n i)
+    simpa [ProtocolSpec.append, FinVec.append_eq_fin_append, Fin.append_left]
+      using T (Fin.castAdd n i)
 
 /-- The second half of a transcript for a concatenated protocol -/
 def snd (T : FullTranscript (pSpec₁ ++ₚ pSpec₂)) : FullTranscript pSpec₂ :=
   fun i => by
-    simpa [ProtocolSpec.append, Fin.append_right] using T (Fin.natAdd m i)
+    simpa [ProtocolSpec.append, FinVec.append_eq_fin_append, Fin.append_right]
+      using T (Fin.natAdd m i)
 
 @[simp]
 theorem append_fst (T₁ : FullTranscript pSpec₁) (T₂ : FullTranscript pSpec₂) :
     (T₁ ++ₜ T₂).fst = T₁ := by
   funext i
-  simp [fst, append, eqRec_eq_cast]
+  simp [fst, append]; sorry
 
 @[simp]
 theorem append_snd (T₁ : FullTranscript pSpec₁) (T₂ : FullTranscript pSpec₂) :
     (T₁ ++ₜ T₂).snd = T₂ := by
   funext i
-  simp [snd, append, eqRec_eq_cast]
+  simp [snd, append]; sorry
 
 end FullTranscript
 
 def MessageIdx.inl (i : MessageIdx pSpec₁) : MessageIdx (pSpec₁ ++ₚ pSpec₂) :=
-  ⟨Fin.castAdd n i.1, by simpa only [Fin.append_left] using i.2⟩
+  ⟨Fin.castAdd n i.1, by simpa only [FinVec.append_eq_fin_append, Fin.append_left] using i.2⟩
 
 def MessageIdx.inr (i : MessageIdx pSpec₂) : MessageIdx (pSpec₁ ++ₚ pSpec₂) :=
-  ⟨Fin.natAdd m i.1, by simpa only [Fin.append_right] using i.2⟩
+  ⟨Fin.natAdd m i.1, by simpa only [FinVec.append_eq_fin_append, Fin.append_right] using i.2⟩
 
 @[simps!]
 def MessageIdx.sumEquiv :
@@ -195,9 +220,9 @@ def MessageIdx.sumEquiv :
   toFun := Sum.elim (MessageIdx.inl) (MessageIdx.inr)
   invFun := fun ⟨i, h⟩ => by
     by_cases hi : i < m
-    · simp [ProtocolSpec.append, Fin.append, Fin.addCases, hi] at h
+    · simp [FinVec.append_eq_fin_append, Fin.append, Fin.addCases, hi] at h
       exact Sum.inl ⟨⟨i, hi⟩, h⟩
-    · simp [ProtocolSpec.append, Fin.append, Fin.addCases, hi] at h
+    · simp [FinVec.append_eq_fin_append, Fin.append, Fin.addCases, hi] at h
       exact Sum.inr ⟨⟨i - m, by omega⟩, h⟩
   left_inv := fun i => by
     rcases i with ⟨⟨i, isLt⟩, h⟩ | ⟨⟨i, isLt⟩, h⟩ <;>
@@ -208,10 +233,10 @@ def MessageIdx.sumEquiv :
     congr; omega
 
 def ChallengeIdx.inl (i : ChallengeIdx pSpec₁) : ChallengeIdx (pSpec₁ ++ₚ pSpec₂) :=
-  ⟨Fin.castAdd n i.1, by simpa only [Fin.append_left] using i.2⟩
+  ⟨Fin.castAdd n i.1, by simpa only [FinVec.append_eq_fin_append, Fin.append_left] using i.2⟩
 
 def ChallengeIdx.inr (i : ChallengeIdx pSpec₂) : ChallengeIdx (pSpec₁ ++ₚ pSpec₂) :=
-  ⟨Fin.natAdd m i.1, by simpa only [Fin.append_right] using i.2⟩
+  ⟨Fin.natAdd m i.1, by simpa only [FinVec.append_eq_fin_append, Fin.append_right] using i.2⟩
 
 @[simps!]
 def ChallengeIdx.sumEquiv :
@@ -219,9 +244,9 @@ def ChallengeIdx.sumEquiv :
   toFun := Sum.elim (ChallengeIdx.inl) (ChallengeIdx.inr)
   invFun := fun ⟨i, h⟩ => by
     by_cases hi : i < m
-    · simp [ProtocolSpec.append, Fin.append, Fin.addCases, hi] at h
+    · simp [FinVec.append_eq_fin_append, Fin.append, Fin.addCases, hi] at h
       exact Sum.inl ⟨⟨i, hi⟩, h⟩
-    · simp [ProtocolSpec.append, Fin.append, Fin.addCases, hi] at h
+    · simp [FinVec.append_eq_fin_append, Fin.append, Fin.addCases, hi] at h
       exact Sum.inr ⟨⟨i - m, by omega⟩, h⟩
   left_inv := fun i => by
     rcases i with ⟨⟨i, isLt⟩, h⟩ | ⟨⟨i, isLt⟩, h⟩ <;>
@@ -240,11 +265,11 @@ def seqCompose {m : ℕ} {n : Fin m → ℕ} (pSpec : ∀ i, ProtocolSpec (n i))
     ProtocolSpec (∑ i, n i) :=
   Fin.dfoldl m (fun i => ProtocolSpec (∑ j : Fin i, n (j.castLE (by omega))))
     (fun i acc => dcast (by simp [Fin.sum_univ_castSucc, Fin.castLE]) (acc ++ₚ pSpec i))
-      ![]
+      !p[]
 
 @[simp]
 theorem seqCompose_zero {n : ℕ} {pSpec : ProtocolSpec n} :
-    seqCompose (fun _ : Fin 0=> pSpec) = ![] := by
+    seqCompose (fun _ : Fin 0=> pSpec) = !p[] := by
   simp [seqCompose]
 
 /-- Sequential composition of `i + 1` protocol specifications equals the sequential composition of
